theories/Compile.v
@@ -1,0 +1,157 @@
+From MetaCoq Require Import PCUICAstUtils.
+From MetaCoq.Erasure Require Import EAst ESpineView EEtaExpanded EInduction ERemoveParams Erasure EGlobalEnv.
+From Malfunction Require Import Ast.
+From Equations Require Import Equations.
+From Coq Require Import List String Arith Lia.
+Import ListNotations.
+From MetaCoq Require Import MCList.
+
+Section MapiInP.
+  Context {A B : Type}.
+
+  Equations mapi_InP (l : list A) (n : nat) (f : nat -> forall x : A, In x l -> B) : list B :=
+  mapi_InP nil n _ := nil;
+  mapi_InP (cons x xs) n f := cons (f n x _) (mapi_InP xs (S n) (fun n x inx => f n x _)).
+End MapiInP.
+
+Lemma mapi_InP_spec' {A B : Type} (f : nat -> A -> B) (l : list A) n :
+  mapi_InP l n (fun n (x : A) _ => f n x) = mapi_rec f l n.
+Proof.
+  remember (fun n (x : A) _ => f n x) as g.
+  funelim (mapi_InP l n g); simpl. reflexivity.
+  simp mapi_InP.
+  f_equal. 
+  now rewrite (H f0).
+Qed.
+
+Lemma mapi_InP_spec {A B : Type} (f : nat -> A -> B) (l : list A) :
+  mapi_InP l 0 (fun n (x : A) _ => f n x) = mapi f l.
+Proof.
+  eapply mapi_InP_spec'.
+Qed.
+
+Section Compile.
+  Context (Σ : global_declarations).
+
+  Definition int_of_nat n := Uint63.of_Z (Coq.ZArith.BinInt.Z.of_nat n).
+
+  Import TermSpineView.
+
+  Definition Mapply_ '(e, l) :=
+      match l with [] => e | _ => Mapply (e, l) end.
+
+  Definition Mlambda_ '(e, l) :=
+      match e with [] => l | _ => Mlambda (e, l) end.
+
+  Definition Mbox :=
+    Mlet ([Recursive [("reccall"%string, Mlambda (["_"%string], Mvar 1) )]], Mvar 0).
+
+  Definition lookup_record_projs (e : global_declarations) (ind : Kernames.inductive) : option (list Kernames.ident) :=
+    match lookup_inductive e ind with
+    | Some (mdecl, idecl) => Some (map proj_name idecl.(ind_projs))
+    | None => None
+    end.
+
+  Equations? compile (t: term) : Malfunction.Ast.t
+  by wf t (fun x y : EAst.term => size x < size y) :=
+  | e with TermSpineView.view e := {
+    | tRel n => Mvar n
+    | tBox => Mbox
+    | tLambda nm bod => Mlambda ([bytestring.String.to_string (BasicAst.string_of_name nm)], compile bod)
+    | tLetIn nm dfn bod => Mlet ([Named (bytestring.String.to_string (BasicAst.string_of_name nm), compile dfn)], compile bod)
+    | tApp fn args napp nnil =>
+        Mapply_ (compile fn, map_InP args (fun x H => compile x))
+    | tConst nm => Mglobal (bytestring.String.to_string (Kernames.string_of_kername nm))
+    | tConstruct i m args => Mblock (int_of_nat m, map_InP args (fun x H => compile x))
+    | tCase i mch brs =>
+        Mswitch (compile mch, mapi_InP brs 0 (fun i '(nms, b) H => ([Malfunction.Tag (int_of_nat i)], Mapply_ (Mlambda_ (rev_map (fun nm => bytestring.String.to_string (BasicAst.string_of_name nm)) nms, compile b),
+                                                                                                        mapi (fun i _ => Mfield (int_of_nat i, compile mch)) (rev nms)))))
+    | tFix mfix idx =>
+        let bodies := map_InP mfix (fun d H => (bytestring.String.to_string (BasicAst.string_of_name (d.(dname))), compile d.(dbody))) in
+        Mlet ([Recursive bodies], Mvar idx)
+    | tProj (Kernames.mkProjection ind _ nargs) bod with lookup_record_projs Σ ind :=
+      { | Some args =>
+            let len := List.length args in
+            Mfield (int_of_nat (len - 1 - nargs), compile bod)
+        | None => Mstring "Proj" }
+    | tCoFix mfix idx => Mstring "TCofix"
+    | tVar _ => Mstring "tVar"
+    | tEvar _ _ => Mstring "Evar"
+    }.
+  Proof.
+    all: try (cbn; lia).
+    - eapply size_mkApps_f; eauto.
+    - eapply le_lt_trans. 2: eapply size_mkApps_l; eauto. eapply (In_size id size) in H.
+      unfold id in H. change size with (fun x => size x) at 2. lia.
+    - eapply (In_size id size) in H.
+      unfold id in H. change size with (fun x => size x) at 2. lia.
+    - eapply (In_size snd size) in H. cbn in H.
+      lia.
+    - eapply (In_size dbody size) in H. cbn in H. lia.
+  Qed.
+  
+End Compile.
+
+From MetaCoq Require Import ETransform Transform bytestring.
+Import Transform.
+
+Require Malfunction.SemanticsSpec Malfunction.Semantics.
+
+Program Definition block_erasure_pipeline {guard : PCUICWfEnvImpl.abstract_guard_impl} (efl := EWellformed.all_env_flags) :=
+  erasure_pipeline ▷ constructors_as_blocks_transformation (hastrel := eq_refl) (hastbox := eq_refl).
+Next Obligation.
+  intros. cbn. MCUtils.todo "ok"%bs.
+Qed.
+
+Program Definition malfunction_pipeline {guard : PCUICWfEnvImpl.abstract_guard_impl} (efl := EWellformed.all_env_flags) :
+ Transform.t TemplateProgram.template_program Malfunction.t
+             Ast.term Malfunction.t
+             TemplateProgram.eval_template_program
+             (fun _ _ => True) :=
+  block_erasure_pipeline ▷ 
+  _.
+Next Obligation.
+  intros. unshelve econstructor.
+  - exact (fun _ => True).
+  - cbn. intros [Σ t] _. refine (Semantics.named _ (compile Σ t)). exact [].
+  - exact (fun _ => True).
+  - exact (fun _ _ _ _ => True).
+  - exact "malfunction"%bs.
+  - cbn. eauto.
+  - cbn. econstructor. exact (Malfunction.Mvar ""%string). eauto.
+Defined.
+Next Obligation.
+  cbn. intros. eauto.
+Qed.
+
+From Ceres Require Import Ceres.
+From Malfunction Require Import Serialize.
+
+Definition compile_malfunction {cf : config.checker_flags} (p : Ast.Env.program)
+  : String.string :=
+  let p' := run malfunction_pipeline p (MCUtils.todo "wf_env and welltyped term"%bs) in
+  time "Pretty printing"%bs to_string  p'.
+
+From MetaCoq.Template Require Import All Loader.
+
+Fixpoint ack (n m:nat) {struct n} : nat :=
+  match n with
+    | 0 => S m
+    | S p => let fix ackn (m:nat) {struct m} :=
+                 match m with
+                   | 0 => ack p 1
+                   | S q => ack p (ackn q)
+                 end
+             in ackn m
+  end.
+Definition ack35 := (ack 3 5).
+
+MetaCoq Quote Recursively Definition cbv_ack35 :=
+  ltac:(let t:=(eval cbv delta [ack35 ack] in ack35) in exact t).
+Local Open Scope string_scope.
+
+(* MetaCoq Quote Recursively Definition p := ltac:(let plus := eval cbv in plus in *)
+(*                                                 let mult := eval cbv in mult in *)
+(*                                                   let eqb := eval cbv in Nat.eqb in *)
+(*                                                     exact (let six := 6 in eqb (plus (mult six six) six) (mult six (plus six 1)))). *)
+Compute (compile_malfunction cbv_ack35).
