theories/Pipeline.v
@@ -1,0 +1,75 @@
+(* Distributed under the terms of the MIT license. *)
+From Coq Require Import Program ssreflect ssrbool.
+From MetaCoq.Template Require Import Transform bytestring config utils.
+From MetaCoq.PCUIC Require PCUICAst PCUICAstUtils PCUICProgram.
+From MetaCoq.SafeChecker Require Import PCUICErrors PCUICWfEnvImpl.
+From MetaCoq.Erasure Require EAstUtils ErasureFunction ErasureCorrectness EPretty Extract.
+From MetaCoq.Erasure Require Import ETransform EConstructorsAsBlocks.
+
+Import PCUICProgram.
+Import TemplateProgram (template_eta_expand).
+Import PCUICTransform (template_to_pcuic_transform, pcuic_expand_lets_transform).
+
+(* This is the total erasure function +
+  let-expansion of constructor arguments and case branches +
+  shrinking of the global environment dependencies +
+  the optimization that removes all pattern-matches on propositions. *)
+
+Import Transform.
+
+Obligation Tactic := program_simpl.
+
+#[local] Existing Instance extraction_checker_flags.
+
+Import EWcbvEval.
+
+Program Definition block_erasure_pipeline {guard : PCUICWfEnvImpl.abstract_guard_impl} (efl := EWellformed.all_env_flags) :=
+  template_eta_expand ▷
+  (* Casts are removed, application is binary, case annotations are inferred from the global environment *)
+  template_to_pcuic_transform ▷
+  (* Branches of cases are expanded to bind only variables, constructor types are expanded accordingly *)
+  pcuic_expand_lets_transform ▷
+  (* Erasure of proofs terms in Prop and types *)
+  erase_transform ▷
+  (* Simulation of the guarded fixpoint rules with a single unguarded one: 
+    the only "stuck" fixpoints remaining are unapplied. 
+    This translation is a noop on terms and environments.  *)
+  guarded_to_unguarded_fix (wcon := eq_refl) eq_refl ▷
+  (* Remove all constructor parameters *)
+  remove_params_optimization (wcon := eq_refl) ▷ 
+  (* Rebuild the efficient lookup table *)
+  rebuild_wf_env_transform (efl := ERemoveParams.switch_no_params EWellformed.all_env_flags) ▷
+  (* Remove all cases / projections on propositional content *)
+  optimize_prop_discr_optimization (efl := ERemoveParams.switch_no_params EWellformed.all_env_flags) (wcon := eq_refl) (hastrel := eq_refl) (hastbox := eq_refl) ▷
+  (* Rebuild the efficient lookup table *)
+  rebuild_wf_env_transform (efl := EWellformed.all_env_flags) ▷
+  (* Constructors are treated as blocks, not higher-order *)
+  constructors_as_blocks_transformation (hastrel := eq_refl) (hastbox := eq_refl).
+Next Obligation.
+  intros. cbn. MCUtils.todo "ok"%bs.
+Qed.
+Next Obligation.
+  intros. cbn. MCUtils.todo "ok"%bs.
+Qed.
+
+Require Malfunction.SemanticsSpec Malfunction.Semantics.
+Require Import Malfunction.Compile.
+
+Program Definition malfunction_pipeline {guard : PCUICWfEnvImpl.abstract_guard_impl} (efl := EWellformed.all_env_flags) :
+ Transform.t TemplateProgram.template_program Malfunction.t
+             Ast.term Malfunction.t
+             TemplateProgram.eval_template_program
+             (fun _ _ => True) :=
+  block_erasure_pipeline ▷ 
+  _.
+Next Obligation.
+  intros. unshelve econstructor.
+  - exact (fun _ => True).
+  - cbn. intros [Σ t] _. refine (Semantics.named _ (compile Σ t)). exact [].
+  - exact (fun _ => True).
+  - exact (fun _ _ _ _ => True).
+  - exact "malfunction"%bs.
+  - cbn. eauto.
+  - cbn. econstructor. refine (Malfunction.Mvar _). red. econstructor. eauto.
+Defined.
+
