theories/Tests.v
@@ -1,0 +1,35 @@
+From Coq Require Import String.
+From Ceres Require Import Ceres.
+From Malfunction Require Import Pipeline Serialize.
+
+From MetaCoq Require Import ETransform Transform bytestring.
+From MetaCoq.Template Require Import All Loader.
+
+Import Transform.
+
+Definition compile_malfunction {cf : config.checker_flags} (p : Ast.Env.program)
+  : String.string :=
+  let p' := run malfunction_pipeline p (MCUtils.todo "wf_env and welltyped term"%bs) in
+  time "Pretty printing"%bs to_string  p'.
+
+Fixpoint ack (n m:nat) {struct n} : nat :=
+  match n with
+    | 0 => S m
+    | S p => let fix ackn (m:nat) {struct m} :=
+                 match m with
+                   | 0 => ack p 1
+                   | S q => ack p (ackn q)
+                 end
+             in ackn m
+  end.
+Definition ack35 := (ack 3 5).
+
+MetaCoq Quote Recursively Definition cbv_ack35 :=
+  ltac:(let t:=(eval cbv delta in (
+
+                   ack 3 5
+
+               ))
+        in exact t).
+Compute (compile_malfunction cbv_ack35).
+
